examples/map/MapIAAproof.v
@@ -1,5 +1,5 @@
 Require Import Coqlib ITreelib sflib.
-Require Import MapHeader MapASpec MapMSpec MapI MapM MapA ModSim MapIMproof MapMAproof MemA.
+Require Import MapHeader MapASpec MapMSpec MapI MapM MapA MapAA ModSim MapIMproof MapMAproof MapAAAproof MemA.
 Require Import ImpPrelude.
 Require Import Skeleton.
 Require Import PCM IPM.
@@ -37,18 +37,25 @@ Section PROOF.
     (MapInStbMap: forall sk, stb_incl MapAS.Stb (StbMap sk))
     :
     ctx_refines
-      ((MapA.t gi StbMap) ★ (MemA.t gi StbMem), MapA.InitCond ∗∗ MapM.InitCond)
-      ((MapI.t)           ★ (MemA.t gi StbMem), const(emp%I)).
+      ((MapAA.t gi StbMap) ★ (MemA.t gi StbMem), MapA.InitCond ∗∗ MapM.InitCond)
+      ((MapI.t)            ★ (MemA.t gi StbMem), const(emp%I)).
   Proof.
     etrans; cycle 1.
-    - eapply main_adequacy. eapply MapIM.sim.
+    { eapply main_adequacy. eapply MapIM.sim.
       instantiate (1:= const(to_stb MapMS.Stb)).
-      i. split; try refl. unfold MapMS.Stb. unseal "ccr". prove_nodup.
-    - eapply ctxr_frameR.
-      rewrite/__ -{2}(hmod_addc_empty_l MapM.InitCond).
+      i. split; try refl. unfold MapMS.Stb. unseal "ccr". prove_nodup. }
+    etrans; cycle 1.
+    { eapply ctxr_frameR.
+      rewrite <-(hmod_addc_empty_l MapM.InitCond).
       eapply ctxr_cond_frameR.
       eapply main_adequacy. eapply MapMA.sim; eauto.
-      i. split; try refl. unfold MapMS.Stb. unseal "ccr". prove_nodup.
+      i. split; try refl. unfold MapMS.Stb. unseal "ccr". prove_nodup. }
+    { eapply ctxr_frameR.
+      rewrite <-(hmod_addc_empty_l (_ ∗∗ _)).
+      eapply ctxr_cond_frameR.
+      eapply main_adequacy. eapply MapAAA.sim; eauto.
+    }
+  Unshelve. eauto.
   Qed.
 
 End PROOF.
